leanification/Chapter3_GraphTheory.lean
@@ -40,3 +40,4 @@ import Chapter3_GraphTheory.Section3_3.SigmaBlockedWalks
 import Chapter3_GraphTheory.Section3_3.ISigmaSeparation
 import Chapter3_GraphTheory.Section3_3.SigmaSeparationSymmetric
 import Chapter3_GraphTheory.Section3_3.LabelRoman
+import Chapter3_GraphTheory.Section3_3.SigmaOpenPathsWalks
